Insert Missing polynomial (#1)
* small tweaks for complexity library

* -added analysis for TM Rev
-Added subterm property

* updated uptoc

* worked on compiler runtimes

* -integrated necessary size analysis for missing time inv analysis
-refined other polynomial for inv thesis

* added poly-analyses up to (excluding final compiler)

* added time analysis for final Compiler-machine

* filled in missing polynomial for computability-characterisation for inv-thesis from L to TM

theories/TM/L/CompilerBoolFuns/Compiler.v
@@ -1,5 +1,5 @@
 From Undecidability.Shared.Libs.PSL Require Import FinTypes Vectors.
-From Undecidability.L Require Import L_facts LM_heap_def.
+From Undecidability.L Require Import L_facts LM_heap_def UpToCNary.
 
 
 From Coq Require Import List.
@@ -22,18 +22,22 @@ Section APP_right.
     App _.
   
   Lemma APP_right_Spec :
-    { f & forall s1 s2 : term,
+    { f : UpToC (fun '(s1,s2)=>size (compile s1) + size (compile s2)) & forall s1 s2 : term,
     TripleT ≃≃([],[|Contains _ (compile s1);Contains _ (compile s2)|])
-    (f s1 s2) APP_right (fun _ => ≃≃([],[|Contains _ (compile (L.app s1 s2));Void|])) }.
+    (f (s1,s2)) APP_right (fun _ => ≃≃([],[|Contains _ (compile (L.app s1 s2));Void|])) }.
   Proof.
-    evar (f : term -> term -> nat).
-    eexists f. [f]:intros s1 s2.
+    eexists_UpToC f. [f]:refine (fun '(s1,s2) => _).
     intros s1 s2.
     unfold APP_right.
     hsteps_cbn.
     -rewrite app_assoc.  reflexivity.
     -reflexivity.
-    -unfold f. reflexivity.
+    - rewrite !(correct__leUpToC (App_steps_nice _) (_,_)).
+      rewrite Encode_list_hasSize with (xs:=(compile s1 ++ compile s2)%list).
+      rewrite Encode_list_hasSize_app, <- !Encode_list_hasSize. reflexivity.
+    -assert (H': (fun x => 1) <=c (fun '(s1,s2)=>size (compile s1) + size (compile s2))).
+     { eapply upToC_le. intros []. setoid_rewrite Encode_list_hasSize. setoid_rewrite <- Encode_list_hasSize_ge1. nia. }
+    unfold f. unfold sigPro. cbn - ["-" "+"]. smpl_upToC. cbn. all:try smpl_upToC_solve.
   Qed.
  
 
@@ -125,7 +129,7 @@ Opaque MK_isVoid_multi.
 
 From Undecidability Require Import TM.L.Transcode.Boollist_to_Enc.
 From Undecidability Require Import EncBoolsTM_boolList.
-
+From Undecidability.TM.L Require Import SizeBoundsL.
 
 Section mk_init_one.
 
@@ -157,27 +161,44 @@ Section mk_init_one.
 
     
   Lemma M_init_one_Spec :
-    { f & forall (bs:list bool) (ter : L.term),
+    { f : UpToC (fun '(bs,ter)=>length bs + L_facts.size ter + 1) & forall (bs:list bool) (ter : L.term),
     TripleT ≃≃([],[|Custom (eq (encBoolsTM s b bs));Contains _ (compile ter);Void;Void;Void;Void|])
-    (f bs ter) M_init_one (fun _ => ≃≃([],[|Custom (eq (encBoolsTM s b bs));Contains _ (compile (L.app ter (encBoolsL bs)));Void;Void;Void;Void|])) }.
+    (f (bs,ter)) M_init_one (fun _ => ≃≃([],[|Custom (eq (encBoolsTM s b bs));Contains _ (compile (L.app ter (encBoolsL bs)));Void;Void;Void;Void|])) }.
   Proof using H_disj.
-    evar (f : list bool -> term -> nat).
-    eexists f. [f]:intros bs ter.
+    eexists_UpToC f. 
+    { 
+    [f]:refine (fun '(bs,ter) => _).
     intros bs ter.
     unfold M_init_one.
     hstep. { hsteps_cbn. cbn. eapply (projT2 (encBoolsTM2boollist.SpecT _ H_disj)). }
     cbn. intros _. hstep. { hsteps_cbn. cbn. tspec_ext. } 2:reflexivity.
     cbn. intros _. hstep.
     {
-      hsteps_cbn. cbn. eapply ConsequenceT. eapply (projT2 (@BoollistToEnc.SpecT _ _ _) (rev bs)).
+      hsteps_cbn. cbn. eapply ConsequenceT. eapply BoollistToEnc.SpecT with (bs:=rev bs).
       all:cbn. now tspec_ext. now rewrite rev_involutive. reflexivity.
     } 2:reflexivity.
     cbn. intros _. hsteps_cbn.
      now eapply (projT2 (APP_right_Spec)). 1,2:now cbn;tspec_ext.
-     subst f. cbn beta. reflexivity.
+     subst f. cbn beta. cbn beta iota.  reflexivity.
+    }
+    etransitivity.
+    {
+       unfold f. eapply upToC_le with (F:=fun '(bs,ter) => _). intros [bs ter].
+       rewrite (correct__leUpToC (Rev_steps_nice _)).
+       rewrite (correct__leUpToC (BoollistEnc.boollist_size)).
+       do 3 rewrite (correct__leUpToC (correct__UpToC _)).
+       rewrite rev_length.
+       rewrite !size_le_sizeP.
+       unfold sizeP;rewrite !sizeP_size.
+       rewrite (correct__leUpToC size_L_enc_bools).
+       reflexivity.
+    }
+       smpl_upToC_solve.
   Qed.
 
 End  mk_init_one.
+
+
 
 Section mk_init.
 
@@ -189,14 +210,12 @@ Section mk_init.
 
   Variable m k : nat.
 
-  Variable sim : term.
-
   Notation aux n := (Fin.L k (Fin.L m n)) (only parsing).
   Notation auxm n := (Fin.L k (Fin.R 6 n)) (only parsing).
   Notation auxk n := (Fin.R (6 + m) n) (only parsing).
 
-  Fixpoint M_init' k' : (Vector.t (Fin.t k) k') -> pTM (Σ) ^+ unit ((6 + m)+ k).
-  Proof using m s retr_bools sim retr_pro. 
+  Fixpoint M_init' (sim:term) {k'} : (Vector.t (Fin.t k) k') -> pTM (Σ) ^+ unit ((6 + m)+ k).
+  Proof using m s retr_bools retr_pro. 
     simple notypeclasses refine (match k' with
     0 => fun _ => MK_isVoid_multi _ @ [|aux Fin1;aux Fin2;aux Fin3;aux Fin4; aux Fin5|];;
         WriteValue ( (compile sim)) ⇑ retr_pro @ [|aux Fin1|]
@@ -204,15 +223,16 @@ Section mk_init.
     fun ren =>
       _;;M_init_one s retr_pro retr_bools @ [|auxk (ren[@Fin0]);aux Fin1;aux Fin2;aux Fin3;aux Fin4;aux Fin5|]
     end). all:try exact _.
-    2:{apply (M_init' _ (Vector.tl ren)). }
+    2:{apply (M_init' sim _ (Vector.tl ren)). }
   Defined. (* because definition *)
 
 
 
-  Theorem M_init'_SpecT k' (ren :Vector.t (Fin.t k) k') (v:Vector.t (list bool) k):
-  { k &
+  Theorem M_init'_SpecT k' (ren :Vector.t (Fin.t k) k') : 
+  { f : UpToC (fun '(sim,v) => L_facts.size sim + sumn (Vector.to_list (Vector.map (length (A:=bool)) v)) + 1)
+  & forall sim (v:Vector.t (list bool) k),
   TripleT ≃≃([],Vector.const (Custom (eq niltape)) (6+m) ++ Vector.map (fun bs => Custom (eq (encBoolsTM s b bs))) v)
-    k (M_init' ren)
+    (f (sim,v)) (M_init' sim ren)
     (fun _ => ≃≃([],
       ([|Custom (eq niltape);
         Contains retr_pro (compile (Vector.fold_right (fun l_i s => L.app s (encBoolsL l_i)) (select ren v) sim))
@@ -220,24 +240,64 @@ Section mk_init.
   Proof using All.
     depind ren. all:cbn [compile Vector.fold_left M_init' Vector.tl Vector.caseS].
     {
-      eexists. cbn.
-      hstep. hsteps_cbn;cbn. exact (MK_isVoid_multi_SpecT 5). cbn;cleanupParamTM. 2:reflexivity.
-      hsteps_cbn. reflexivity.
-      cleanupParamTM.
-      apply EntailsI. intros t H. eapply tspec_ext. eassumption. easy.
-      intros i. clear - i.
-      repeat (destruct (fin_destruct_S i) as [(i'&->) | ->];[rename i' into i;cbn| ]);try (intros H;exact H).
+      eexists_UpToC f. [f]:refine (fun '(sim,v) => _). 
+      {
+        cbn. intros sim v.
+        hstep. hsteps_cbn;cbn. exact (MK_isVoid_multi_SpecT 5). cbn;cleanupParamTM. 2:reflexivity.
+        hsteps_cbn. reflexivity.
+        cleanupParamTM.
+        apply EntailsI. intros t H. eapply tspec_ext. eassumption. easy.
+        intros i. clear - i.
+        repeat (destruct (fin_destruct_S i) as [(i'&->) | ->];[rename i' into i;cbn| ]);try (intros H;exact H).
+      }
+      unfold f. etransitivity. 
+      {eapply upToC_le with (F:= (fun '(_,_) => _ ));intros []. unfold WriteValue_steps. rewrite !size_le_sizeP. unfold sizeP;rewrite !sizeP_size. reflexivity. }
+      smpl_upToC_solve.
     }
     {
-      eexists. cbn. hstep.
-      3:reflexivity. now apply (projT2 (IHren v)). clear IHren.
-      cbn. intros _. hstep. { cbn. rewrite Vector_nth_R,nth_map'. cbn. eapply (projT2 (M_init_one_Spec H_disj _ _)). }
-      cbn;fold Nat.add;rewrite Nat.eqb_refl;cbn. intros _.
-      apply EntailsI. intros t H. eapply tspec_ext. eassumption. easy.
-      intros i. clear - i. 
-      repeat (destruct (fin_destruct_S i) as [(i'&->) | ->];[rename i' into i;cbn| ]);try (intros H;exact H).
-      rewrite nth_tabulate. destruct (Fin.eqb _ _) eqn:H'. 2:tauto.
-      cbn. eapply Fin.eqb_eq in H' as ->. rewrite Vector_nth_R,nth_map'. cbn. tauto.
+      eexists_UpToC f. [f]:refine (fun '(sim,v) => _).
+      { 
+        cbn. intros sim v.
+        hstep.
+        3:reflexivity. now apply (projT2 IHren). 
+        cbn. intros _. hstep. { cbn. rewrite Vector_nth_R,nth_map'. cbn. eapply (projT2 (M_init_one_Spec H_disj _ _)). }
+        cbn;fold Nat.add;rewrite Nat.eqb_refl;cbn. intros _.
+        apply EntailsI. intros t H. eapply tspec_ext. eassumption. easy.
+        intros i. clear - i. 
+        repeat (destruct (fin_destruct_S i) as [(i'&->) | ->];[rename i' into i;cbn| ]);try (intros H;exact H).
+        rewrite nth_tabulate. destruct (Fin.eqb _ _) eqn:H'. 2:tauto.
+        cbn. eapply Fin.eqb_eq in H' as ->. rewrite Vector_nth_R,nth_map'. cbn. tauto.
+      }
+      unfold f. etransitivity. 
+      {
+        eapply upToC_le with (F:= (fun '(_,_) => _ ));intros [].
+        do 2 rewrite (correct__leUpToC (correct__UpToC _)). reflexivity.
+      }
+      assert (Hnth : forall n h,(fun '(_, x) => | x[@h] |) <=c
+          (fun '(sim, v) =>
+          L_facts.size sim + sumn (Vector.to_list (n:=n) (Vector.map (length (A:=bool)) v)) +
+          1)).
+          {
+          clear. intros. eapply upToC_le;intros [? ?].
+          clear. revert h t0. induction n;intros i v. easy. depelim v. depelim i.
+            now cbn;nia.
+            cbn. rewrite IHn. unfold Vector.to_list. nia.
+          }
+      smpl_upToC.
+      all:try smpl_upToC_solve. now apply Hnth.
+      -clear - Hnth. induction n.
+       +depelim ren;cbn. smpl_upToC_solve.
+       +depelim ren;cbn.
+        etransitivity.   
+        *eapply upToC_le with (F:= (fun '(_,_) => _ ));intros []. unfold select in IHn.  rewrite (correct__leUpToC (IHn ren) (_,_)). reflexivity.
+        *smpl_upToC. all:try smpl_upToC_solve.
+         etransitivity.
+         {
+           eapply upToC_le with (F:= (fun '(_,_) => _ ));intros [? ?].
+           change (encBoolsL t0[@h]) with (Extract.enc t0[@h]).
+           rewrite (correct__leUpToC size_L_enc_bools). reflexivity.
+         }
+           smpl_upToC. apply Hnth. smpl_upToC_solve.
     }
   Qed.
 
@@ -262,27 +322,37 @@ Section mk_init.
 
 
 
-  Definition M_init : pTM (Σ) ^+ unit ((6 + m)+ k) :=
-    M_init' startRen.
+  Definition M_init sim : pTM (Σ) ^+ unit ((6 + m)+ k) :=
+    M_init' sim startRen.
 
     
-  Theorem M_init_SpecT (v:Vector.t (list bool) k):
-  { k &
+  Theorem M_init_SpecT:
+  { f : UpToC (fun '(sim,v) => L_facts.size sim + sumn (Vector.to_list (Vector.map (length (A:=bool)) v)) + 1)
+    & forall sim (v:Vector.t (list bool) k),
   TripleT ≃≃([],Vector.const (Custom (eq niltape)) (6+m) ++ Vector.map (fun bs => Custom (eq (encBoolsTM s b bs))) v)
-    k M_init
+    (f (sim,v)) (M_init sim)
     (fun _ => ≃≃([],
       ([|Custom (eq niltape);
         Contains retr_pro (compile (Vector.fold_left (fun s l_i => L.app s (encBoolsL l_i)) sim v));
          Void;Void;Void;Void|]
          ++Vector.const (Custom (eq niltape)) m) ++ Vector.map (fun bs => Custom (eq (encBoolsTM s b bs))) v))}.
   Proof using H_disj.
-    eexists. unfold M_init.
-    eapply ConsequenceT. eapply (projT2 (M_init'_SpecT _ _)). reflexivity. 2:reflexivity.
+    eexists_UpToC f. [f]:refine (fun '(sim,v) => _).
+    intros. 
+    unfold M_init.
+    eapply ConsequenceT. eapply (projT2 (M_init'_SpecT _)). reflexivity. 2:unfold f;reflexivity.
     cbn. intros _.
     rewrite vector_fold_left_right with (v:=v), <- (startRen_spec v).
     apply EntailsI. intros t H. eapply tspec_ext. eassumption. easy.
     intros i. clear - i. 
     repeat (destruct (fin_destruct_S i) as [(i'&->) | ->];[rename i' into i;cbn| ]);try (intros H;exact H).
+    unfold f;cbn beta.
+    etransitivity.
+    {
+       eapply upToC_le with (F:= fun '(x,y)=>_);intros []. cbn. 
+      setoid_rewrite (correct__leUpToC (correct__UpToC _)). reflexivity.
+    }
+    smpl_upToC_solve.
   Qed.
 
 
@@ -304,22 +374,26 @@ Section conv_output.
     Boollist2encBoolsTM.M s b _ @ [|Fin2;Fin1;Fin3|].
 
   
-  Theorem M_out_SpecT bs:
-    { k &
+  Theorem M_out_SpecT :
+    { f : UpToC (fun bs => length bs + 1) & forall bs,
     TripleT ≃≃([],[|Contains _ (compile (encBoolsL bs));Custom (eq niltape);Void;Void|])
-      k M_out
+      (f bs) M_out
       (fun _ => ≃≃([],
         ([|Custom (fun _ => True); Custom (eq (encBoolsTM s b bs)); Void;Void|])))}.
   Proof.
-    eexists. unfold M_out. hsteps_cbn;cbn.
+    eexists_UpToC f. [f]:refine (fun bs => _).
+    intro bs.
+    unfold M_out. hsteps_cbn;cbn.
     -eapply (projT2 (@EncToBoollist.SpecT _ _ _)).
     -eapply (projT2 (Boollist2encBoolsTM.SpecT _ _ _)).
     - cbn. rewrite rev_involutive. tspec_ext. easy.
-    -reflexivity.
+    -unfold f.  setoid_rewrite (correct__leUpToC (correct__UpToC _)). rewrite rev_length. reflexivity.
+    -unfold f. smpl_upToC_solve.
   Qed.
 
 End conv_output.
 
+From Undecidability.TM.L.HeapInterpreter Require UnfoldClosBounds.
 
 Section main.
 
@@ -331,8 +405,8 @@ Section main.
   Hypothesis Hscl : closed s.
 
   Variable Hs1 : (forall v, forall m : list bool,
-   R v m <->
-   L.eval (Vector.fold_left (fun (s0 : term) (n : list bool) => L.app s0 (encBoolsL n)) s v) (encBoolsL m)).
+   L.eval (Vector.fold_left (fun (s0 : term) (n : list bool) => L.app s0 (encBoolsL n)) s v) (encBoolsL m)
+   -> R v m).
 
   Variable Hs2 : (forall v, forall o : term,
                      L.eval (Vector.fold_left (n := k) (fun (s0 : term) (n : list bool) => L.app s0 (encBoolsL n)) s v) o ->
@@ -377,9 +451,9 @@ Section main.
        M_main
       (fun _ t => exists m, t ≃≃ ([R v m]%list,
         (Custom (eq (encBoolsTM sym_s sym_b m)):::Vector.const (Custom (fun _ => True)) _))).
-  Proof  using Hscl Hs2 Hs1.
+  Proof  using Hscl Hs1 Hs2.
     unfold M_main.
-    hstep. { eapply TripleT_Triple,(projT2 (M_init_SpecT syms_diff _ _ _ _ _)). }
+    hstep. { eapply TripleT_Triple,(projT2 (M_init_SpecT syms_diff _ _ _ _)). }
     cbn. intros _.
     start_TM.
     hstep. {hsteps_cbn;cbn. eapply TripleT_Triple. exact (MK_isVoid_multi_SpecT 9). }
@@ -391,7 +465,7 @@ Section main.
     hintros Heval%eval_iff. specialize (Hs2 Heval) as (res&->). 
     unfold_abbrev.
     eapply Triple_exists_con. eexists res. 
-    hstep. { eapply Consequence_pre. eapply TripleT_Triple. refine (projT2 (M_out_SpecT _ _ _ _ res)). cbn. reflexivity. }
+    hstep. { eapply Consequence_pre. eapply TripleT_Triple. refine (projT2 (M_out_SpecT _ _ _ _) res). cbn. reflexivity. }
     cbn;cleanupParamTM. intros _.
     apply Hs1 in Heval.
     eapply EntailsI. intros tin [[] Hin]%tspecE.
@@ -399,35 +473,79 @@ Section main.
     intros i. specialize (Hin i). destruct_fin i;try exact Logic.I;cbn in *.
     now simpl_vector. eassumption.
   Qed.
+End main.
 
-Theorem M_main_SpecT v res:
-  R v res -> exists k__steps,
-  TripleT ≃≃([],Vector.const (Custom (eq niltape)) (S n_main) ++ Vector.map (fun bs => Custom (eq (encBoolsTM sym_s sym_b bs))) v)
-  k__steps M_main
-    (fun _ => ≃≃([],Custom (eq (encBoolsTM sym_s sym_b res)):::Vector.const (Custom (fun _ => True)) _)).
-Proof  using Hscl Hs2 Hs1.
-  unfold M_main. intros ?.
-  apply Hs1 in H as H%eval_iff. eapply eval_evalIn in H as [? H].
-  (* edestruct EvalL.SpecT'. 2:eassumption. now eapply closed_compiler_helper. *)
-  eexists. 
-  hstep. { eapply (projT2 (M_init_SpecT syms_diff _ _ _ _ _)). } 2:reflexivity.
+Import UpToCNary.
+
+
+
+Polymorphic Lemma upToC_mul_descend_nary (domain : list Type) (f g f' g': Rarrow domain nat):
+  Uncurry f <=c Uncurry f'
+  -> Uncurry g <=c Uncurry g'
+  -> Fun' (fun x => App f x * App g x)
+    <=c Fun' (fun x => App f' x * App g' x).
+Proof.
+  prove_nary upToC_mul_descend. 
+Qed.
+
+Theorem M_main_SpecT k s (Hscl : closed s):
+  { f : UpToC (fun '(i,m_r,m_v) => (i+1)*(i+m_v+1)*((m_v+1)*(i+1) + m_r)) & 
+  forall i v res,
+    (Vector.fold_left (fun (s0 : term) (n : list bool) => L.app s0 (encBoolsL n)) s v) ⇓(i) (encBoolsL res)  ->
+    TripleT ≃≃([],Vector.const (Custom (eq niltape)) (S n_main) ++ Vector.map (fun bs => Custom (eq (encBoolsTM sym_s sym_b bs))) v)
+    (f (i,length res,sumn (Vector.to_list (Vector.map (length (A:=bool)) v)))) (M_main k s)
+      (fun _ => ≃≃([],Custom (eq (encBoolsTM sym_s sym_b res)):::Vector.const (Custom (fun _ => True)) (13+S k)))}.
+Proof.
+  eexists_UpToC f. [f]:refine (fun '(i,m_r,m_v) => _). 
+  intros ? ? ? Red. unfold M_main.
+  eapply ConsequenceT_pre. 2:reflexivity.
+  { 
+  hstep. { eapply (projT2 (M_init_SpecT syms_diff _ _ _ _)). }
+  2:{ set (f' := f__UpToC _). pose (H' := correct__UpToC _ :f' <=c _). rewrite (correct__leUpToC H'). subst f' H'; cbn beta;reflexivity. }
   cbn. intros _.
   start_TM.
   hstep. {hsteps_cbn;cbn. exact (MK_isVoid_multi_SpecT 9). } 2:reflexivity.
   cbn;cleanupParamTM. intros _.
-  hstep. { eapply LiftTapes_SpecT. now smpl_dupfree. cbn. apply @EvalL.SpecT. }
+  hstep. { eapply LiftTapes_SpecT. now smpl_dupfree. cbn. unshelve apply EvalL.SpecT. 3:now eapply closed_compiler_helper. 3:easy. }
   cbn;cleanupParamTM.
   intros _.
-  hstep. now refine (projT2 (M_out_SpecT _ _ _ _ res)). 
+  hstep. now refine (projT2 (M_out_SpecT _ _ _ _) res). 
   cbn;cleanupParamTM. intros _. 
   eapply EntailsI. intros tin [[] Hin]%tspecE.
   eapply tspecI;cbn. easy.
-  intros i. specialize (Hin i). destruct_fin i;try exact Logic.I;cbn in *.
-  now simpl_vector. eassumption. reflexivity.
-  Unshelve. 3:easy. now eapply closed_compiler_helper.
-Qed.
+  intros j. specialize (Hin j). destruct_fin j;try exact Logic.I;cbn in *.
+  now simpl_vector. eassumption. cbn beta.
+  set (l:= EvalL.steps _ _).
+  pose (Hl:= proj2_sig UnfoldClosBounds.EvalL_steps_nice' _ _ _ _ _ : l <= _ ). 
+  rewrite Hl.   setoid_rewrite (correct__leUpToC (correct__UpToC _)) at 1. reflexivity.
+  } 
+  set (f' := L_facts.size
+      (Vector.fold_left _ _ _)). pose (H':= correct__leUpToC (size_fold_app k) (s,v) : f' <= _).
+      cbn in H'. setoid_rewrite H'. clear f' H'.
+  rewrite (LargestVar_fold s v) at 1.
+  change (encBoolsL) with (Extract.enc (X:=list bool)).
+  rewrite (correct__leUpToC size_L_enc_bools res).
 
-End main.
+  unfold f;cbn beta iota.
+  set (m_s:= L_facts.size s). set (m_v:= sumn (Vector.to_list (Vector.map (length (A:=bool)) v))). 
+  set (m_r := length res).
+  reflexivity.
+  unfold f. cbn - ["+" "*"]. clear.
+  assert ( (fun _ => 1) <=c (fun '(i, m_r,m_v) => (i + 1) * (i + m_v+1) * ((m_v + 1) * (i + 1) + m_r))) by smpl_upToC_solve.
+  smpl_upToC.
+  1,3:now smpl_upToC_solve.
+  eapply leUpToC_proper_eq with (x:=fun '(i, m_r,m_v) => _) (x0:=fun '(i, m_r,m_v) => _).
+  { intros [[]]. rewrite <- !Nat.mul_assoc. reflexivity. }
+  { intros [[]]. rewrite <- !Nat.mul_assoc. reflexivity. }
+  nary simple apply upToC_mul_descend_nary. reflexivity.
+  nary simple apply upToC_mul_descend_nary. now smpl_upToC_solve.
+  smpl_upToC.
+  2,3:smpl_upToC_solve.
+  transitivity ((fun '(t', x) => let '(t'0, x0) := t' in (0*x0)+(x + 1) * (t'0 + 1))).
+  1,2:cbn.
+  nary simple apply upToC_mul_descend_nary; now smpl_upToC_solve.
+  smpl_upToC_solve.
+Qed.
 
 Theorem compiler_correct {k} (R : Vector.t (list bool) k -> (list bool) -> Prop) :
   L_bool_computable_closed R -> TM_bool_computable_hoare' R.
@@ -438,5 +556,6 @@ Proof.
   eexists _, _, sym_s, sym_b. split. eapply syms_diff. exists (M_main k sim).
   intros v. split.
   - eapply M_main_Spec. easy. all:firstorder.
-  - eapply M_main_SpecT. easy. all:firstorder.
+  - intros. edestruct eval_evalIn. now apply eval_iff,Hsim.
+    eexists. eapply (projT2 (M_main_SpecT _ cs)). easy.
 Qed.
