theories/L/AbstractMachines/LargestVar.v
@@ -1,4 +1,5 @@
-From Undecidability.L.Datatypes Require Import LProd LNat LTerm.
+From Undecidability.L Require Import Util.Subterm.
+From Undecidability.L.Datatypes Require Import LProd LNat LTerm LBool List_enc.
 
 Fixpoint largestVar (s:term) : nat :=
   match s with
@@ -7,6 +8,17 @@ Fixpoint largestVar (s:term) : nat :=
   | lam s => largestVar s
   end.
 
+Lemma subterm_largestVar s s' :
+subterm s s' -> largestVar s <= largestVar s'.
+Proof.
+  induction 1;cbn;Lia.nia.
+Qed.
+
+Lemma largestVar_size s :
+  largestVar s <= size s.
+Proof.
+  induction s;cbn;Lia.lia.
+Qed.
 
 Lemma largestVar_prod X Y `{Rx : encodable X} {Ry : encodable Y} (w:X*Y):
   largestVar (enc w) = max (largestVar (enc (fst w))) (largestVar (enc (snd w))).
@@ -29,8 +41,25 @@ Proof.
   all:try Lia.lia.
 Qed.
 
-Lemma largestVar_size s :
-  largestVar s <= size s.
+Lemma largestVar_bool (b:bool):
+  largestVar (enc b) <= 1.
 Proof.
-  induction s;cbn;Lia.lia.
+  destruct b;cbv. all:easy.
+Qed.
+
+Lemma largestVar_list X {R:encodable X} (xs:list X):
+  largestVar (enc xs) <= max (list_max (map (fun x => largestVar (enc x)) xs)) 1.
+Proof.
+  unfold enc,encodable_list_enc.
+  induction xs. now cbv.
+  cbn.
+  rewrite IHxs. unfold enc,list_max. nia.
+Qed.
+
+Lemma largestVar_bools (bs:list bool):
+  largestVar (enc bs) <= 1.
+Proof.
+  rewrite largestVar_list.
+  specialize list_max_le with (n:=1) as [_ H]. rewrite H. easy.
+  eapply Forall_forall. intros ? (?&<-&?)%in_map_iff. eapply largestVar_bool.
 Qed.
