theories/TM/L/HeapInterpreter/LMBounds.v
@@ -4,7 +4,7 @@ From Undecidability Require Import TM.PrettyBounds.PrettyBounds.
 From Undecidability Require Import TM.PrettyBounds.BaseCode.
 From Undecidability Require Import LM_heap_def TM.PrettyBounds.MaxList.
 
-From Undecidability.TM.L  Require Import CaseCom Alphabets JumpTargetTM LookupTM StepTM.
+From Undecidability.TM.L  Require Import CaseCom Alphabets JumpTargetTM LookupTM StepTM SizeBoundsL.
 
 
 From Undecidability.TM.L Require Import StepTM M_LHeapInterpreter.
@@ -39,61 +39,6 @@ Smpl Add 12
      | [ |- (match _ with appT => _ | _ => _ end) <=(_) _ ] =>
        let H := fresh in (eapply dominatedWith_match_Tok;[intros H..|intros ? H]);try rewrite !H
      end : domWith_match.
-
-
-(** ** Sizes for (atomic) commands *)
-
-Lemma size_ACom_singleton (t : ACom) :
-  size [ACom2Com t] = 4.
-Proof. destruct t; cbn; cbv; reflexivity. Qed.
-
-Lemma size_ACom_singleton' (t : ACom) :
-  size [t] = 3.
-Proof. destruct t; cbn; cbv; reflexivity. Qed.
-
-Lemma size_ACom (t : ACom) :
-  size t = 1.
-Proof. unfold size. destruct t; cbn; reflexivity. Qed.
-
-Lemma size_ACom' (t : ACom) :
-  size (ACom2Com t) = 2.
-Proof. unfold size. destruct t; cbn; reflexivity. Qed.
-
-Lemma size_Var (n : nat) :
-  size (varT n) = 2 + n.
-Proof. unfold size. cbn. simpl_list. rewrite repeat_length. cbn. lia. Qed.
-
-Lemma size_nat' (n : nat) :
-  size (varT n) = 1 + size n.
-Proof. unfold size. cbn. simpl_list. rewrite repeat_length. cbn. lia. Qed.
-
-Lemma Encode_Com_hasSize_ge1 (t : Tok) :
-  1 <= size t.
-Proof. unfold size. destruct t; auto. unfold Encode_Heap. cbn. simpl_list. all: cbn; lia. Qed.
-
-Lemma size_Com_singleton (t : Tok) :
-  size [t] = 2 + size t.
-Proof. unfold size. destruct t; cbn; try lia. simpl_list. rewrite repeat_length. cbn. lia. Qed.
-
-Lemma Encode_Pro_hasSize_ge1 (P : Pro) :
-  1 <= size P.
-Proof. setoid_rewrite Encode_list_hasSize. apply Encode_list_hasSize_ge1. Qed.
-
-Lemma Encode_Pro_hasSize_ge_length (P : Pro) :
-  length P <= Encode_list_size _ P.
-Proof.
-  induction P.
-  - cbn. lia.
-  - cbn. rewrite IHP. lia.
-Qed.
-
-Lemma Encode_Heap_hasSize_ge_length (H : Heap) :
-  length H <= Encode_list_size _ H.
-Proof.
-  induction H.
-  - cbn. lia.
-  - cbn. rewrite IHlist. lia.
-Qed.
 
 (** ** JumpTarget *)
 
@@ -386,39 +331,6 @@ End JumpTarget_steps_nice.
 
 
 (** ** LM Lookup *)
-
-
-Lemma Encode_Clos_hasSize (g : HClos) :
-  size g = fst g + Encode_list_size _ (snd g) + 1.
-Proof.
-  destruct g as (a,P); cbn.
-  setoid_rewrite Encode_pair_hasSize; unfold Encode_pair_size.
-  setoid_rewrite Encode_nat_hasSize.
-  setoid_rewrite Encode_list_hasSize.
-  lia.
-Qed.
-
-Lemma Encode_Clos_hasSize' (g : HClos) :
-  size g = size (fst g) + Encode_list_size _ (snd g).
-Proof.
-  destruct g as (a,P); cbn.
-  setoid_rewrite Encode_pair_hasSize; unfold Encode_pair_size.
-  setoid_rewrite Encode_nat_hasSize.
-  setoid_rewrite Encode_list_hasSize.
-  lia.
-Qed.
-
-Lemma Encode_Clos_hasSize_ge1 (g : HClos) :
-  1 <= size g.
-Proof. rewrite Encode_Clos_hasSize. lia. Qed.
-
-Lemma Encode_HEntr_hasSize_ge1 (e : HEntr) :
-  1 <= size e.
-Proof. setoid_rewrite Encode_option_hasSize. apply Encode_option_hasSize_ge1. Qed.
-
-Lemma Encode_Heap_hasSize_ge1 (H : Heap) :
-  1 <= size H.
-Proof. setoid_rewrite Encode_list_hasSize. apply Encode_list_hasSize_ge1. Qed.
 
 
 Module LM_Lookup_nice.
